slicker proof of associativity for products
Signed-off-by: Ali Caglayan <alizter@gmail.com>

theories/WildCat/Products.v
@@ -171,7 +171,7 @@ Class HasBinaryProducts (A : Type) `{Is1Cat A} := {
 (** *** Symmetry of products *)
 
 Section Symmetry.
-
+  
   (** The requirement of having all binary products can be weakened further to having specific binary products, but it is not clear this is a useful generality. *)
   Context {A : Type} `{HasEquivs A} `{!HasBinaryProducts A}.
 
@@ -202,86 +202,6 @@ Section Symmetry.
   Defined. 
 
 End Symmetry.
-
-(** *** Associativity of products *)
-
-Section Associativity.
-
-  Context {A : Type} `{HasEquivs A} `{!HasBinaryProducts A}.
-
-  Definition cat_prod_assoc (x y z : A)
-    : cat_prod x (cat_prod y z) $-> cat_prod (cat_prod x y) z
-    := cat_prod_corec (cat_prod_corec cat_pr1 (cat_pr1 $o cat_pr2)) (cat_pr2 $o cat_pr2).
-
-  Definition cat_prod_assoc_inv (x y z : A)
-    : cat_prod (cat_prod x y) z $-> cat_prod x (cat_prod y z)
-    := cat_prod_corec (cat_pr1 $o cat_pr1) (cat_prod_corec (cat_pr2 $o cat_pr1) cat_pr2).
-
-  Lemma cat_prod_assoc_cat_prod_assoc_inv (x y z : A)
-    : cat_prod_assoc x y z $o cat_prod_assoc_inv x y z $== Id _.
-  Proof.
-    unfold cat_prod_assoc, cat_prod_assoc_inv.
-    apply cat_prod_pr_eta.
-    - refine ((cat_assoc _ _ _)^$ $@ _).
-      refine (cat_prod_beta_pr1 _ _ $@R _ $@ _).
-      apply cat_prod_pr_eta.
-      + refine ((cat_assoc _ _ _)^$ $@ _).
-        refine (cat_prod_beta_pr1 _ _ $@R _ $@ _).
-        refine (cat_prod_beta_pr1 _ _ $@ _).
-        exact (_ $@L (cat_idr _)^$).
-      + refine ((cat_assoc _ _ _)^$ $@ _).
-        refine (cat_prod_beta_pr2 _ _ $@R _ $@ _).
-        refine (cat_assoc _ _ _ $@ _).
-        refine (_ $@L (cat_prod_beta_pr2 _ _) $@ _).
-        refine (cat_prod_beta_pr1 _ _ $@ _).
-        exact (_ $@L (cat_idr _)^$).
-    - refine ((cat_assoc _ _ _)^$ $@ _).
-      refine (cat_prod_beta_pr2 _ _ $@R _ $@ _).
-      refine (cat_assoc _ _ _ $@ _).
-      refine (_ $@L (cat_prod_beta_pr2 _ _) $@ _).
-      refine (cat_prod_beta_pr2 _ _ $@ _).
-      exact (cat_idr _)^$.
-  Defined.
-
-  Lemma cat_prod_assoc_inv_cat_prod_assoc (x y z : A)
-    : cat_prod_assoc_inv x y z $o cat_prod_assoc x y z $== Id _.
-  Proof.
-    unfold cat_prod_assoc, cat_prod_assoc_inv.
-    apply cat_prod_pr_eta.
-    - refine ((cat_assoc _ _ _)^$ $@ _).
-      refine (cat_prod_beta_pr1 _ _ $@R _ $@ _).
-      refine (cat_assoc _ _ _ $@ _).
-      refine (_ $@L (cat_prod_beta_pr1 _ _) $@ _).
-      refine (cat_prod_beta_pr1 _ _ $@ _).
-      exact (cat_idr _)^$.
-    - refine ((cat_assoc _ _ _)^$ $@ _).
-      refine (cat_prod_beta_pr2 _ _ $@R _ $@ _).
-      apply cat_prod_pr_eta.
-      + refine ((cat_assoc _ _ _)^$ $@ _).
-        refine (cat_prod_beta_pr1 _ _ $@R _ $@ _).
-        refine (cat_assoc _ _ _ $@ _).
-        refine (_ $@L (cat_prod_beta_pr1 _ _) $@ _).
-        refine (cat_prod_beta_pr2 _ _ $@ _).
-        exact (_ $@L (cat_idr _)^$).
-      + refine ((cat_assoc _ _ _)^$ $@ _).
-        refine (cat_prod_beta_pr2 _ _ $@R _ $@ _).
-        refine (cat_prod_beta_pr2 _ _ $@ _).
-        exact (_ $@L (cat_idr _)^$).
-  Defined.
-
-  Lemma cate_prod_assoc (x y z : A)
-    : cat_prod x (cat_prod y z) $<~> cat_prod (cat_prod x y) z.
-  Proof.
-    snrapply cate_adjointify.
-    - apply cat_prod_assoc.
-    - apply cat_prod_assoc_inv.
-    - apply cat_prod_assoc_cat_prod_assoc_inv.
-    - apply cat_prod_assoc_inv_cat_prod_assoc.
-  Defined.
-
-End Associativity.
-
-(** *** Unit of products *)
 
 (** *** Product functor *)
 
@@ -408,3 +328,64 @@ Proof.
     + exact (p x).
     + exact (q x).
 Defined.
+
+(** *** Associativity of products *)
+
+Section Associativity.
+
+  Context {A : Type} `{HasEquivs A} `{!HasBinaryProducts A}.
+
+  Definition cat_prod_twist (x y z : A)
+    : cat_prod x (cat_prod y z) $-> cat_prod y (cat_prod x z).
+  Proof.
+    apply cat_prod_corec.
+    - exact (cat_pr1 $o cat_pr2).
+    - exact (fmap (fun y => cat_prod x y) cat_pr2).
+  Defined.
+  
+  Lemma cat_prod_twist_cat_prod_twist (x y z : A)
+    : cat_prod_twist x y z $o cat_prod_twist y x z $== Id _.
+  Proof.
+    unfold cat_prod_twist.
+    apply cat_prod_pr_eta.
+    - refine ((cat_assoc _ _ _)^$ $@ _).
+      refine (cat_prod_beta_pr1 _ _ $@R _ $@ _).
+      refine (cat_assoc _ _ _ $@ _).
+      refine (_ $@L cat_prod_beta_pr2 _ _ $@ _).
+      refine (cat_prod_beta_pr1 _ _ $@ _).
+      exact (cat_idr _)^$.
+    - refine ((cat_assoc _ _ _)^$ $@ _).
+      refine (cat_prod_beta_pr2 _ _ $@R _ $@ _).
+      apply cat_prod_pr_eta.
+      + refine ((cat_assoc _ _ _)^$ $@ _).
+        refine (cat_prod_beta_pr1 _ _ $@R _ $@ _).
+        refine (cat_prod_beta_pr1 _ _ $@ _).
+        refine (_ $@L _).
+        exact (cat_idr _)^$.
+      + refine ((cat_assoc _ _ _)^$ $@ _).
+        refine (cat_prod_beta_pr2 _ _ $@R _ $@ _).
+        refine (cat_assoc _ _ _ $@ _).
+        refine (_ $@L cat_prod_beta_pr2 _ _ $@ _).
+        refine (cat_prod_beta_pr2 _ _ $@ _).
+        refine (_ $@L _).
+        exact (cat_idr _)^$.
+  Defined.
+
+  Definition cate_prod_twist (x y z : A)
+    : cat_prod x (cat_prod y z) $<~> cat_prod y (cat_prod x z).
+  Proof.
+    snrapply cate_adjointify.
+    1,2: apply cat_prod_twist.
+    1,2: apply cat_prod_twist_cat_prod_twist.
+  Defined.
+
+  Lemma cate_prod_assoc (x y z : A)
+    : cat_prod x (cat_prod y z) $<~> cat_prod (cat_prod x y) z.
+  Proof.
+    refine (cate_prod_swap _ _ $oE _).
+    refine (cate_prod_twist _ _ _ $oE _).
+    refine (emap (fun y => cat_prod x y) _).
+    exact (cate_prod_swap _ _).
+  Defined.
+
+End Associativity.
